Work on substitution lore

FreydSSA/Terminator/Fun/Subst.lean
@@ -8,7 +8,7 @@ variable {φ : Type u₁} {ν : Type u₂} {κ : Type u₃} {α : Type u₄} [Φ
 inductive FLCtx.SubstBot
   : WithBot (FLabel ν (Ty α)) → USubst φ ν →  WithBot (FLabel ν (Ty α)) → Type _
   | bot (σ Γ) : SubstBot ⊥ σ Γ
-  | subst (hσ : FCtx.Subst Γ σ Δ) (A : Ty α) : SubstBot (↑(FLabel.mk Γ A)) σ (↑(FLabel.mk Δ A))
+  | subst {Γ Δ : FLabel ν (Ty α)} (hσ : FCtx.Subst Γ.live σ Δ.live) (hparam : Γ.param = Δ.param) : SubstBot (↑Γ) σ (↑Δ)
 
 -- TODO: composition, other such nonsense
 
@@ -20,7 +20,25 @@ def FLCtx.Subst (L : FLCtx κ ν (Ty α)) (σ : USubst φ ν) (K : FLCtx κ ν (
 inductive FLCtx.PSubstBot
   : WithBot (FLabel ν (Ty α)) → USubst φ ν →  WithBot (FLabel ν (Ty α)) → Type _
   | bot (σ) : PSubstBot ⊥ σ ⊥
-  | subst (hσ : FCtx.Subst Γ σ Δ) (A : Ty α) : PSubstBot (↑(FLabel.mk Γ A)) σ (↑(FLabel.mk Δ A))
+  | subst {Γ Δ : FLabel ν (Ty α)} (hσ : FCtx.Subst Γ.live σ Δ.live) (hparam : Γ.param = Δ.param) : PSubstBot (↑Γ) σ (↑Δ)
+
+theorem FLCtx.PSubstBot.bot_mp {Γ : WithBot (FLabel ν (Ty α))} {σ : USubst φ ν} {Δ : WithBot (FLabel ν (Ty α))}
+  (hσ : PSubstBot Γ σ Δ) : Γ = ⊥ → Δ = ⊥
+  := λh => by
+    cases hσ with
+    | bot => rfl
+    | subst => cases h
+
+theorem FLCtx.PSubstBot.bot_mpr {Γ : WithBot (FLabel ν (Ty α))} {σ : USubst φ ν} {Δ : WithBot (FLabel ν (Ty α))}
+  (hσ : PSubstBot Γ σ Δ) : Δ = ⊥ → Γ = ⊥
+  := λh => by
+    cases hσ with
+    | bot => rfl
+    | subst => cases h
+
+theorem FLCtx.PSubstBot.param_eq {Γ : FLabel ν (Ty α)} {σ : USubst φ ν} {Δ : FLabel ν (Ty α)}
+  (hσ : @PSubstBot _ ν α Φ (↑Γ) σ (↑Δ)) : Γ.param = Δ.param
+  := by cases hσ; assumption
 
 def FLCtx.PSubstBot.toSubstBot
   {Γ : WithBot (FLabel ν (Ty α))} {σ : USubst φ ν} {Δ : WithBot (FLabel ν (Ty α))}
@@ -31,9 +49,75 @@ def FLCtx.PSubstBot.toSubstBot
 def FLCtx.PSubst (L : FLCtx κ ν (Ty α)) (σ : USubst φ ν) (K : FLCtx κ ν (Ty α))
   := ∀x, PSubstBot (L x) σ (K x)
 
+theorem FLCtx.PSubst.bot_mp {L : FLCtx κ ν (Ty α)} {σ : USubst φ ν} {K : FLCtx κ ν (Ty α)}
+  (hσ : L.PSubst σ K) (x : κ) : L x = ⊥ → K x = ⊥
+  := (hσ x).bot_mp
+
+theorem FLCtx.PSubst.bot_mpr {L : FLCtx κ ν (Ty α)} {σ : USubst φ ν} {K : FLCtx κ ν (Ty α)}
+  (hσ : L.PSubst σ K) (x : κ) : K x = ⊥ → L x = ⊥
+  := (hσ x).bot_mpr
+
+-- def FLCtx.PSubst.lsup
+--   {L₁ L₂ : FLCtx κ ν (Ty α)} {σ : USubst φ ν} {K₁ K₂ : FLCtx κ ν (Ty α)}
+--   (hσ₁ : L₁.PSubst σ K₁) (hσ₂ : L₂.PSubst σ K₂) : (L₁.lsup L₂).PSubst σ (K₁.lsup K₂)
+--   := λx => by
+--     simp only [lsup_app, lsup_bot]
+--     split
+--     . rename_i he
+--       split
+--       . exact hσ₂ x
+--       . rename_i c
+--         exact (c $ hσ₁.bot_mp _ he).elim
+--       . rename_i he' _
+--         simp [hσ₁.bot_mp _ he] at he'
+--     . rename_i he c
+--       split
+--       . rename_i he'
+--         exact (c $ hσ₁.bot_mpr _ he').elim
+--       . exact hσ₁ x
+--       . rename_i he'
+--         simp [hσ₂.bot_mp _ he] at he'
+--     . rename_i Γ₁ Γ₂ hLe₁ hLe₂
+--       split
+--       . rename_i he
+--         simp [hσ₁.bot_mpr _ he] at hLe₁
+--       . rename_i he _
+--         simp [hσ₂.bot_mpr _ he] at hLe₂
+--       . rename_i Δ₁ Δ₂ hKe₁ hKe₂
+--         let h₁ := hKe₁ ▸ hLe₁ ▸ hσ₁ x;
+--         let h₂ := hKe₂ ▸ hLe₂ ▸ hσ₂ x;
+--         cases h₁
+--         constructor
+--         sorry -- TODO: lsup substitution
+--         assumption
+--         -- apply PSubstBot.subst
+
+-- TODO: PSubst preserves compatibility
+
 def FLCtx.PSubst.toSubst {L : FLCtx κ ν (Ty α)} {σ : USubst φ ν} {K : FLCtx κ ν (Ty α)}
   (hσ : L.PSubst σ K) : L.Subst σ K
   := λx => (hσ x).toSubstBot
+
+def FCtx.Subst.toPSingleton {Γ : FCtx ν (Ty α)} {σ : USubst φ ν} {Δ : FCtx ν (Ty α)}
+  (x : κ) (hσ : Γ.Subst σ Δ) (param : Ty α) : (Γ.toSingleton x param).PSubst σ (Δ.toSingleton x param)
+  := λy => by
+    if h : y = x then
+      simp only [toSingleton, h, FLCtx.singleton_app, ↓reduceIte]
+      constructor
+      assumption
+      rfl
+    else
+      simp only [toSingleton, h, FLCtx.singleton_app, ↓reduceIte]
+      constructor
+
+-- def UTerminator.FWfM.subst {Γ : FCtx ν (Ty α)} {t : UTerminator φ ν κ}
+--   (hσ : Γ.Subst σ Δ)
+--   : t.FWfM Δ L → (L' : FLCtx κ ν (Ty α)) × (t.rewrite σ).FWfM Γ L' × (L'.PSubst σ L)
+--   | br _ de rfl => ⟨_, br _ (de.subst hσ) rfl, hσ.toPSingleton _ _⟩
+--   | ite de ds dt h rfl =>
+--     let ⟨Ls', ds', σs'⟩ := ds.subst hσ;
+--     let ⟨Lt', dt', σt'⟩ := dt.subst hσ;
+--     ⟨_, ite (de.subst hσ) ds' dt' sorry rfl, σs'.lsup σt'⟩
 
 -- TODO: PSubst for FWfM
 
